coq/SystemFProp.v
@@ -118,9 +118,10 @@ Proof with eauto.
       assert (exists t0, t1 = ttabs t0).
       eapply canonical_forms_tabs; eauto.
       destruct H0; subst.
-      exists ([0 := T2] x)...
+      inversion H1. inversion H0.
+      exists ([0 := T2] t)...
     SCase "t1 also steps".
-      inversion H. exists (ttapp x T2)...
+      inversion H0. exists (ttapp x T2)...
 Qed.
 
 (* [] *)
@@ -217,12 +218,20 @@ Inductive type_appears_free_in_type : nat -> ty -> Prop :=
       type_appears_free_in_type X (TArrow T1 T2)
   | afit_arrow2 : forall X T1 T2,
       type_appears_free_in_type X T2 ->
-      type_appears_free_in_type X (TArrow T1 T2).
+      type_appears_free_in_type X (TArrow T1 T2)
+  | afit_univ1 : forall X T1 T2,
+      type_appears_free_in_type X T1 ->
+      type_appears_free_in_type X (TUniv T1 T2)
+  | afit_univ2 : forall X T1 T2,
+      type_appears_free_in_type X T2 ->
+      type_appears_free_in_type (X + 1) (TUniv T1 T2).
+
 
 Tactic Notation "afit_cases" tactic(first) ident(c) :=
   first;
   [ Case_aux c "afit_var"
-  | Case_aux c "afit_arrow1" | Case_aux c "afit_arrow2" ].
+  | Case_aux c "afit_arrow1" | Case_aux c "afit_arrow2"
+  | Case_aux c "afit_univ1" | Case_aux c "afit_univ2" ].
 
 Hint Constructors type_appears_free_in_type.
 
@@ -277,10 +286,41 @@ Definition closed_type_term (t:tm) :=
     and if we know [t] is well typed in context [Gamma], then it must
     be the case that [Gamma] assigns a type to [x]. *)
 
+Lemma free_in_context_type : forall X T Gamma,
+   type_appears_free_in_type X T ->
+   wf_ty Gamma T ->
+   get_tvar Gamma X = true.
+Proof.
+  intros X T Gamma H Hwf. generalize dependent Gamma.
+  generalize dependent X. induction T; intros.
+  Case "TVar".
+    simpl in Hwf. trivial.  
+
+afit_cases (induction H) Case; intros.
+  Case "afit_var".
+    simpl in Hwf. trivial.
+  Case "afit_arrow1".
+    apply IHtype_appears_free_in_type. simpl in Hwf. inversion Hwf.
+    trivial.
+  Case "afit_arrow2".
+    apply IHtype_appears_free_in_type. simpl in Hwf. inversion Hwf.
+    trivial.
+  Case "afit_univ1".
+    apply IHtype_appears_free_in_type. simpl in Hwf. inversion Hwf.
+    trivial.
+  Case "afit_univ2".
+    simpl in Hwf. inversion Hwf. 
+
+    apply IHtype_appears_free_in_type in H1. trivial.
+    
+
+inversion Hwf.
+    trivial.
+
 Lemma free_in_context : forall x t T Gamma,
    term_appears_free_in_term x t ->
    Gamma |- t \in T ->
-   exists T', get_var Gamma x = Some T'.
+   exists T', get_var Gamma x = Some T' /\ wf_type Gamma T'.
 
 (** _Proof_: We show, by induction on the proof that [x] appears free
       in [t], that, for all contexts [Gamma], if [t] is well typed
@@ -318,8 +358,8 @@ Proof.
          intros; try solve [inversion H0; eauto].
   Case "afi_abs".
     inversion H1; subst.
-    apply IHterm_appears_free_in_term in H7.
-    inversion H7. inversion H2. destruct (eq_id_dec x y); subst.
+    apply IHterm_appears_free_in_term in H8.
+    inversion H8. inversion H2. destruct (eq_id_dec x y); subst.
     apply ex_falso_quodlibet; apply H; reflexivity.
     exists x0; assumption.
   Case "afi_tabs".
@@ -354,11 +394,46 @@ Proof.
   Case "tabs".
     admit.
   Case "ttapp".
-    eapply IHt. apply H4. inversion Hc; subst. apply H2.
+    eapply IHt. apply H5. inversion Hc; subst. apply H2.
   Case "ttabs".
     admit.
 Qed.
 (** [] *)
+
+Lemma extension_typing : forall Gamma Gamma' X,
+  get_tvar Gamma X = get_tvar Gamma' X ->
+  get_tvar (ext_tvar Gamma) X = get_tvar (ext_tvar Gamma') X.
+Proof.
+  intros. generalize dependent Gamma'.
+  induction Gamma; intros. trivial.
+  admit. admit. admit.
+Admitted.
+
+Lemma context_invariance_type : forall Gamma Gamma' T,
+  wf_ty Gamma T ->
+  (forall X, type_appears_free_in_type X T ->
+             get_tvar Gamma X = get_tvar Gamma' X) ->
+  wf_ty Gamma' T.
+Proof.
+  intros Gamma Gamma' T Hwf H. generalize dependent Gamma. generalize dependent Gamma'.
+  induction T; intros; simpl; simpl in Hwf.
+  Case "TVar".
+    rewrite <- H. trivial. constructor.
+  Case "TArrow".
+    inversion Hwf. split.
+    SCase "wf_ty T1".
+      apply IHT1 with Gamma. trivial. intros. apply H. constructor. trivial.
+    SCase "wf_ty T2".
+      apply IHT2 with Gamma. trivial. intros. apply H. apply afit_arrow2. trivial.
+  Case "TUniv".      
+    inversion Hwf. split.
+    SCase "wf_ty".
+      apply IHT1 with Gamma. trivial. intros. apply H. constructor. trivial.
+    SCase "wf_ty T2".
+      apply IHT2 with (ext_tvar Gamma). trivial. intros. 
+      apply extension_typing. apply H. admit.
+Admitted.
+
 
 (** Sometimes, when we have a proof [Gamma |- t : T], we will need to
     replace [Gamma] by a different context [Gamma'].  When is it safe
@@ -371,6 +446,8 @@ Lemma context_invariance_term : forall Gamma Gamma' t T,
      Gamma |- t \in T  ->
      (forall x, term_appears_free_in_term x t ->
                 get_var Gamma x = get_var Gamma' x) ->
+     (forall X, type_appears_free_in_type X T ->
+                get_tvar Gamma X = get_tvar Gamma' X) ->
      Gamma' |- t \in T.
 
 (** _Proof_: By induction on the derivation of [Gamma |- t \in T].
@@ -424,6 +501,8 @@ Proof with eauto.
     apply T_Var. rewrite <- H0...
   Case "T_Abs".
     apply T_Abs.
+    eapply context_invariance_type. apply H.
+    intros. apply H2...
     apply IHhas_type. intros x1 Hafi.
     (* the only tricky step... the [Gamma'] we use to 
        instantiate is [extend Gamma x T11] *)
@@ -432,35 +511,103 @@ Proof with eauto.
       repeat (rewrite eq_id)...
     SCase "x0 <> x1".
       repeat (rewrite neq_id)...
+    intros. simpl. apply H2. apply afit_arrow2. trivial.
   Case "T_App".
-    apply T_App with T11...
+    apply T_App with T11. apply IHhas_type1. intros. apply H1.
+    constructor. trivial. 
+    intros. admit. admit.
   Case "T_TAbs".
     apply T_TAbs.
     apply IHhas_type. intros x1 Hafi. simpl.
     rewrite H0. reflexivity.
     apply afi_tabs...
+    admit.
   Case "T_TApp".
-    eapply T_TApp. apply IHhas_type...
+    admit. (*eapply T_TApp. IHhas_type... *)
 Qed.
 
 
-Lemma typing_weakening : forall Gamma Gamma' t T n,
-  Gamma  |- t \in T ->
-  Gamma' |- shift_typ n t \in tshift n T.
+Lemma wf_empty_novars : forall T,
+  wf_ty empty T ->
+  closed_type T.
 Proof.
-  intros. generalize dependent n. generalize dependent T.
-  t_cases (induction t) Case; 
-  intros; inversion H; subst.
+  intros T H. unfold closed_type. intros X Ht. induction T.
+  Case "TVar".
+    inversion H; subst.
+  Case "TArrow".
+    inversion Ht; subst. apply IHT1. inversion H; trivial. trivial.
+    apply IHT2. inversion H; trivial. trivial.
+  Case "TUniv".
+    inversion Ht. inversion H. apply IHT1.
+     trivial. trivial. admit.
+
+Qed.
+
+Fixpoint num_tvar_bindings (Gamma:context) : nat :=
+  match Gamma with
+    | empty => 0
+    | ext_var Gamma' _ _ => num_tvar_bindings Gamma'
+    | ext_tvar Gamma' => 1 + num_tvar_bindings Gamma'
+  end.
+
+Lemma shifting_type : forall Gamma U n,
+  wf_ty Gamma U ->
+  num_tvar_bindings Gamma = n ->
+  tshift n U = U.
+Admitted.
+
+Lemma well_formed_type : forall Gamma v U,
+  Gamma |- v \in U ->
+  wf_ty Gamma U.
+Admitted.
+
+Lemma shifting_v : forall Gamma v U n,
+  Gamma |- v \in U ->
+  num_tvar_bindings Gamma = n ->
+  shift_typ n v = v.
+Proof.
+  intros Gamma v U n Ht Hn. generalize dependent n.
+  generalize dependent Gamma. generalize dependent U.
+  t_cases (induction v) Case;
+  intros U Gamma Ht n Hn; inversion Ht. 
   Case "tvar".
-    inversion H2.
+    trivial.
   Case "tapp".
-    simpl. eapply T_App with (tshift n T11).
-    assert (TArrow (tshift n T11) (tshift n T) = tshift n (TArrow T11 T)) by trivial.
-    rewrite H0. apply IHt1. trivial. apply IHt2. trivial.
+    simpl. rewrite IHv1 with (TArrow T11 U) Gamma n; trivial.
+    rewrite IHv2 with T11 Gamma n; 
+    trivial.
   Case "tabs".
-    simpl. apply T_Abs. eapply IHt. 
+    simpl. rename t into T. 
+    admit. admit. admit.
+Admitted.
 
+Lemma typing_weakening_one : forall Gamma t T,
+  Gamma |- t \in T ->
+  ext_tvar Gamma |- shift_typ 1 t \in tshift 1 T.
+Admitted.
 
+Lemma typing_weakening : forall t T n,
+  empty |- t \in T ->
+  empty |- shift_typ n t \in tshift n T.
+Proof.
+Admitted. 
+ (*intros Gamma t T n. generalize dependent n. generalize dependent T. 
+  generalize dependent Gamma. 
+  t_cases (induction t) Case; intros Gamma T Ht n.
+  Case "tvar".
+    inversion Ht; subst. inversion H1.
+  Case "tapp".
+    inversion Ht; subst. simpl. 
+    
+ trivial. simpl. split.
+    
+
+ unfold wf_ty. apply IHt2. trivial.
+  Case "tabs".
+    admit.
+  Case "ttapp".
+    simpl. assert (tshift n ([0 := t0]T12) = [0 := tshift n t0](tshift n T12)).
+      symmetry. rewrite subst_type_in_type_correct. constructor.
 
     simpl. rename T into 
 
@@ -469,7 +616,7 @@ admit.
     simpl. constructor. apply IHt. 
 
 unfold shift_teapply T_TApp.
-
+*)
 (** Now we come to the conceptual heart of the proof that reduction
     preserves types -- namely, the observation that _substitution_
     preserves types.
@@ -570,6 +717,7 @@ Proof with eauto.
       eapply context_invariance_term. apply Ht. intros x Hcontra.
       destruct (free_in_context _ _ T empty Hcontra) as [T' HT']...
       inversion HT'.
+      intros X Hcontra. des
     SCase "x<>y".
       apply T_Var. simpl in H2; rewrite neq_id in H2...
   Case "tabs".
@@ -591,7 +739,7 @@ Proof with eauto.
           simpl; repeat (rewrite neq_id)...
   Case "ttabs".
     apply T_TAbs. apply IHt with (tshift 0 U). 
-
+    apply typing_weakening_one in Ht.
     eapply context_invariance_term...
     intros. simpl. destruct (eq_id_dec x0 x). trivial.
     trivial.
@@ -1520,6 +1668,8 @@ Proof.
     apply IHappears_free_in in H7.
     rewrite extend_neq in H7; assumption.
 Qed.
+
+
 
 
 Lemma context_invariance : forall Gamma Gamma' t T,
